src/Crypto/RSAEncryption.dfy
@@ -47,14 +47,14 @@ module {:extern "RSAEncryption"} RSAEncryption {
             ensures RSAWfDK(padding, dk)
             ensures IsRSAKeypair(padding, ek, dk)
 
-        static function method {:extern "RSADecrypt"} RSADecrypt(padding : RSAPaddingMode, dk : seq<uint8>, c : seq<uint8>) : Option<seq<uint8>>
+        static function method {:extern "RSADecrypt"} RSADecrypt(padding : RSAPaddingMode, dk : seq<uint8>, c : seq<uint8>) : Result<seq<uint8>>
             // requires RSAWfCtx(padding, c) -- there should be a runtime way to establish this. or maybe not?
             requires RSAWfDK(padding, dk) // similarly how should I validate the key is well formed
 
-        static method {:extern "RSAEncrypt"} RSAEncrypt(padding: RSAPaddingMode, ek : seq<uint8>, msg : seq<uint8>) returns (c : Option<seq<uint8>>)
+        static method {:extern "RSAEncrypt"} RSAEncrypt(padding: RSAPaddingMode, ek : seq<uint8>, msg : seq<uint8>) returns (res : Result<seq<uint8>>)
             requires RSAWfEK(padding, ek) // todo: be able to validate this at runtime
-            ensures c.Some? ==> RSAWfCtx(padding, c.get)
-            ensures c.Some? ==> forall dk :: IsRSAKeypair(padding,ek, dk) ==> RSAWfDK(padding,dk) ==> RSADecrypt(padding, dk, c.get) == Some(msg)
+            ensures res.Success? ==> RSAWfCtx(padding, res.value)
+            ensures res.Success? ==> forall dk :: IsRSAKeypair(padding, ek, dk) ==> RSAWfDK(padding, dk) ==> RSADecrypt(padding, dk, res.value) == Success(msg)
 
     }
 
